v2/lakefile.lean
@@ -7,5 +7,8 @@ package lscV2 where
 require mathlib from git
   "https://github.com/leanprover-community/mathlib4" @ "v4.30.0"
 
+require evmyul from git
+  "https://github.com/prevostc/EVMYulLean.git" @ "65124bfc495bd253dc8a615bb55d9cc7e432efa9"
+
 lean_lib LscV2 where
   globs := #[Glob.submodules `LscV2]
