docs/inspiration.md
@@ -4,3 +4,29 @@ https://fe-lang.org/
 evm-smith
 https://leonardoalt.github.io/evm-smith
 https://x.com/leonardoalt/status/2069826134661898442
+
+move lang
+https://certik.substack.com/p/formal-verification-the-move-language
+
+TamaSwap / Tama Tools / Verity
+https://x.com/boredGenius/status/2060094478946558139
+https://tama.tools/
+https://veritylang.com/
+
+Nethermind's Clear
+https://github.com/NethermindEth/Clear
+https://www.nethermind.io/blog/clear-prove-anything-about-your-solidity-smart-contracts
+
+
+Rocq of solidity
+https://formal-land.github.io/rocq-of-solidity/
+https://github.com/formal-land/rocq-of-solidity
+
+K-EVM
+https://github.com/runtimeverification/evm-semantics
+
+Nethermind's EVMYulLean
+https://github.com/NethermindEth/EVMYulLean
+
+Certora
+https://github.com/Layr-Labs/eigenlayer-contracts/tree/main/certora
